code and comment improoved

Matching.v
@@ -2,35 +2,26 @@
 (* -----------------Description----------------------------------------------------------
 
 This file contains useful definitions and basic properties of fundamental concepts 
-about auctions such as matching, maximum matching (MM), individual rational matching (IR), uniform matching, fair matching etc. This file also contains results on matchings, IR matchings, uniform matchings.
+about auctions such as matching, maximum matching (MM), individual rational matching (IR), 
+uniform matching, fair matching etc. This file also contains results on matchings, 
+IR matchings, uniform matchings.
 
-Definition All_matchable := In all the bid-ask pairs, bid price is greater or equal to ask price.
 
-Definition matching := All_matchable and there is no duplicate in the bids of M and no duplicate in asks of M.
+    Terms          <==>     Explanations
+    -----------------------------------------------------
+    All_matchable M        Every bid-ask pair in M are matchable
+    matching M             All_matchable M && NoDup B_M && NoDup A_M              
+    matching_in B A M      matching M && B_M [<=] B && A_M [<=] A
+    Is_MM M B A            M is maximal matching for B and A
+    rational m             bid_of m  >= tp m >= ask_of m
+    Is_IR M                forall m, In n M -> rational m    
+    Uniform M              all bid-ask pairs in M is traded at single price        
+    fair_on_bids B M       M is fair on all bids (i.e. B)
+    fair_on_asks A M       M is fair on all asks (i.e. A) 
+    Is_fair M B A          M is fair on B and A
 
-Definition matching_in := M is matching and bids of M is subset of bids and asks of M is subset of asks.
-
-Definition Is_MM :=size of M is largest amongs the size of all other possible matchings.
-
-Definition rational :=trade price of a bid-ask pair is between the ask price and bid price of the pair.
-
-Definition Is_IR := Each bid-asks pair is rational.
-
-Definition Uniform (M : list fill_type) := The trade price for each bid-ask pair is same.
-
-Definition fair_on_bids := If a bid b is part of matching then all the bids above b must be part of matching.
-
-Definition fair_on_asks := If an ask a is part of matching then all the asks below a must be part of matching.
- 
-Definition Is_fair :=  A matching is fair on bids as well as fair on asks.
-
-Some important results:
-
-Lemma matching_elim9 : matching M ->  matching (delete m M).
-
-Lemma Is_IR_intro : rational m -> Is_IR M -> Is_IR (m::M).
-
-Lemma Uniform_intro : Uniform M -> Uniform (delete m M).
+Most of the results in this file contains the introduction and elimination rules 
+for all the above defined notions.
 
 -----------------------------------------------------------------------------*)
 
@@ -56,14 +47,15 @@ Definition all_matchable (M:list fill_type) := forallb (fun m =>
  (ask_of m) <=? (bid_of m)) M.
 
 Lemma all_matchableP (M:list fill_type): reflect (All_matchable M) (all_matchable M).
-Proof. {  apply reflect_intro.  unfold Prop_bool_eq. split. 
-{
-induction M. intros. simpl. auto. intros. simpl. apply /andP. split.
-apply /leP. unfold All_matchable in H. apply H. auto.  assert (H1: All_matchable M). revert H. unfold All_matchable. simpl. auto.  apply IHM in H1. eauto. }
-{ induction M. intros. unfold All_matchable. intros. destruct H0. 
-simpl. intros. move /andP in H. destruct H. unfold All_matchable. intros. 
-destruct H1. move /leP in H. subst a. exact. eapply IHM in H0. 
-unfold All_matchable in H0. eapply H0 in H1. exact. } } Qed.
+Proof. {  apply reflect_intro.  unfold Prop_bool_eq. split.
+          { induction M. intros. simpl. auto. intros. simpl. apply /andP. split.
+            apply /leP. unfold All_matchable in H. apply H. auto.
+            assert (H1: All_matchable M).
+            revert H. unfold All_matchable. simpl. auto.  apply IHM in H1. eauto. }
+          { induction M. intros. unfold All_matchable. intros. destruct H0.
+            simpl. intros. move /andP in H. destruct H. unfold All_matchable. intros. 
+            destruct H1. move /leP in H. subst a. exact. eapply IHM in H0. 
+            unfold All_matchable in H0. eapply H0 in H1. exact. } } Qed.
 
 Definition matching (M: list fill_type):=
   (All_matchable M) /\ (NoDup (bids_of M)) /\ (NoDup (asks_of M)).
@@ -129,80 +121,108 @@ Lemma matching_elim2 (M: list fill_type): matching M -> NoDup (asks_of M).
 Proof. intro H. unfold matching in H. destruct H. destruct H0. exact. Qed.
 
 Lemma matching_elim3 (M: list fill_type): matching M -> NoDup M.
-Proof. { intro H. destruct H. destruct H0. induction M as [|m].  { auto. } {
-constructor. intro H2. assert (H4: In (bid_of m) (bids_of M)). eauto.
-simpl in H0. assert (H5: ~In (bid_of m) (bids_of M)). eauto. contradiction.
-apply IHM. all: eauto. } } Qed.
+Proof. { intro H. destruct H. destruct H0.
+         induction M as [|m].
+         { auto. }
+         { constructor. intro H2. assert (H4: In (bid_of m) (bids_of M)). eauto.
+           simpl in H0. assert (H5: ~In (bid_of m) (bids_of M)). eauto. contradiction.
+           apply IHM. all: eauto. } } Qed.
 
 
 Lemma matching_elim4 (m: fill_type) (M: list fill_type): matching (m::M) ->
                                                          ~ In (ask_of m) (asks_of M).
-Proof. intros. unfold matching in H. destruct H. destruct H0. simpl in H1.
-eapply nodup_elim2 in H1. exact. Qed.
+Proof. { intros. unfold matching in H. destruct H. destruct H0. simpl in H1.
+         eapply nodup_elim2 in H1. exact. } Qed.
 
 Lemma matching_elim5 (m: fill_type) (M: list fill_type): matching (m::M) ->
                                                          ~ In (bid_of m) (bids_of M).
-Proof.  intros. unfold matching in H. destruct H. destruct H0. simpl in H0.
-eapply nodup_elim2 in H0. exact. Qed.
+Proof. { intros. unfold matching in H. destruct H. destruct H0. simpl in H0.
+         eapply nodup_elim2 in H0. exact. } Qed.
 
 Lemma matching_elim6 (m: fill_type) (M: list fill_type): matching (m::M) -> matching M.
-Proof. intros. unfold matching in H. destruct H. destruct H0. unfold matching.
-split. eapply All_matchable_elim1. eauto. split. eauto. eauto. Qed.
+Proof. { intros. unfold matching in H. destruct H. destruct H0. unfold matching.
+         split. eapply All_matchable_elim1. eauto. split. eauto. eauto. } Qed.
 
 Lemma matching_elim14 (m1 m2: fill_type) (M: list fill_type): matching M -> In m1 M -> In m2 M ->
                                                               m1 <> m2 -> bid_of m1 <> bid_of m2.
-Proof. { induction M.  { intros. destruct H0. } 
-{ intros.  destruct H. destruct H3. destruct H1;destruct H0. 
-{ subst m1. subst m2. destruct H2. exact. }
-{ subst a. simpl in H4.
-assert (H5: In (bid_of m1) (bids_of M)). eauto. 
-assert (H6: ~ In (bid_of m2) (bids_of M)). eauto.
-intro h7. rewrite h7 in H5. contradiction. } 
-{ subst a. simpl in H4.
-assert (H5: In (bid_of m2) (bids_of M)). eauto. 
-assert (H6: ~ In (bid_of m1) (bids_of M)). eauto.
-intro h7. rewrite h7 in H6. contradiction. }
-{ apply IHM. unfold matching;eauto. all: exact. } } } Qed.
+Proof. { induction M.
+         { intros. destruct H0. }
+         { intros.  destruct H. destruct H3. destruct H1;destruct H0.
+           { subst m1. subst m2. destruct H2. exact. }
+           { subst a. simpl in H4.
+             assert (H5: In (bid_of m1) (bids_of M)). eauto. 
+             assert (H6: ~ In (bid_of m2) (bids_of M)). eauto.
+             intro h7. rewrite h7 in H5. contradiction. } 
+           { subst a. simpl in H4.
+             assert (H5: In (bid_of m2) (bids_of M)). eauto. 
+             assert (H6: ~ In (bid_of m1) (bids_of M)). eauto.
+             intro h7. rewrite h7 in H6. contradiction. }
+           { apply IHM. unfold matching;eauto. all: exact. } } } Qed.
 
 Lemma matching_elim15 (m1 m2: fill_type) (M: list fill_type): matching M -> In m1 M -> In m2 M ->
                                                               m1 <> m2 -> ask_of m1 <> ask_of m2.
-Proof.  { induction M.  { intros. destruct H0. } 
-{ intros.  destruct H. destruct H3. destruct H1;destruct H0. 
-{ subst m1. subst m2. destruct H2. exact. }
-{ subst a. simpl in H4.
-assert (H5: In (ask_of m1) (asks_of M)). eauto. 
-assert (H6: ~ In (ask_of m2) (asks_of M)). eauto.
-intro h7. rewrite h7 in H5. contradiction. } 
-{ subst a. simpl in H4.
-assert (H5: In (ask_of m2) (asks_of M)). eauto. 
-assert (H6: ~ In (ask_of m1) (asks_of M)). eauto.
-intro h7. rewrite h7 in H6. contradiction. }
-{ apply IHM. unfold matching;eauto. all: exact. } } } Qed.
+Proof.  { induction M.
+          { intros. destruct H0. } 
+          { intros.  destruct H. destruct H3. destruct H1;destruct H0. 
+            { subst m1. subst m2. destruct H2. exact. }
+            { subst a. simpl in H4.
+              assert (H5: In (ask_of m1) (asks_of M)). eauto. 
+              assert (H6: ~ In (ask_of m2) (asks_of M)). eauto.
+              intro h7. rewrite h7 in H5. contradiction. } 
+            { subst a. simpl in H4.
+              assert (H5: In (ask_of m2) (asks_of M)). eauto. 
+              assert (H6: ~ In (ask_of m1) (asks_of M)). eauto.
+              intro h7. rewrite h7 in H6. contradiction. }
+            { apply IHM. unfold matching;eauto. all: exact. } } } Qed.
 
 
 
 Lemma matching_elim7 (m: fill_type) (M: list fill_type): In m M -> matching M ->
                                                          ~ In (ask_of m) (asks_of (delete m M)).
-Proof.  { intros H1 H2. unfold matching in H2. destruct H2. destruct H0.
-intro H3. assert (H4: exists m', (In m' (delete m M))/\ (ask_of m = ask_of m')). eauto. destruct H4 as [m' H4]. destruct H4 as [H4 H5]. assert (H6: In m' M). eapply included_elim2. eapply included_elim4. apply included_intro2. exact H1. apply included_intro2. exact H4. apply included_refl. assert (H7: m'<>m). cut (NoDup M). { intro. eapply delete_elim2. exact H7. exact H4. } apply matching_elim3. unfold matching. auto. eapply matching_elim15 in H7. symmetry in H5. contradiction. instantiate (1:=M). unfold matching. auto. exact. exact. } Qed.
+Proof.  { intros H1 H2. unfold matching in H2.
+          destruct H2. destruct H0.
+          intro H3.
+          assert (H4: exists m', (In m' (delete m M))/\ (ask_of m = ask_of m')).
+          eauto. destruct H4 as [m' H4]. destruct H4 as [H4 H5].
+          assert (H6: In m' M). eapply included_elim2. eapply included_elim4.
+          apply included_intro2. exact H1. apply included_intro2. exact H4.
+          apply included_refl. assert (H7: m'<>m).
+          cut (NoDup M).
+          { intro. eapply delete_elim2. exact H7. exact H4. }
+          apply matching_elim3. unfold matching. auto.
+          eapply matching_elim15 in H7. symmetry in H5.
+          contradiction. instantiate (1:=M).
+          unfold matching. auto. exact. exact. } Qed.
  
   
 
 Lemma matching_elim8 (m: fill_type) (M: list fill_type): In m M -> matching M ->
                                                          ~ In (bid_of m) (bids_of (delete m M)).
 Proof.  { intros H1 H2. unfold matching in H2. destruct H2. destruct H0.
-intro H3. assert (H4: exists m', (In m' (delete m M))/\ (bid_of m = bid_of m')). eauto. destruct H4 as [m' H4]. destruct H4 as [H4 H5]. assert (H6: In m' M). eauto. assert (H7: m'<>m). cut (NoDup M). eauto. apply matching_elim3.
-unfold matching. auto. eapply matching_elim14 in H7. symmetry in H5. contradiction. instantiate (1:=M). unfold matching. auto. exact. exact. } Qed.
+          intro H3.
+          assert (H4: exists m', (In m' (delete m M))/\ (bid_of m = bid_of m')). eauto.
+          destruct H4 as [m' H4]. destruct H4 as [H4 H5].
+          assert (H6: In m' M). eauto. assert (H7: m'<>m).
+          cut (NoDup M). eauto. apply matching_elim3.
+          unfold matching. auto. eapply matching_elim14 in H7.
+          symmetry in H5. contradiction. instantiate (1:=M).
+          unfold matching. auto. exact. exact. } Qed.
 
 
 
 Lemma matching_elim9 (m: fill_type) (M: list fill_type): matching M ->  matching (delete m M).
-Proof. intros H. unfold matching in H. destruct H. destruct H0. unfold matching. split. 
-{ eauto. } split.
-{  assert (H2: included (delete m M) (M)). eapply included_elim4a. eapply included_M_imp_included_bids in H2. eapply nodup_included_nodup in H2.
-all: exact. }
-{ assert (H2: included (delete m M) (M)). eapply included_elim4a. eapply included_M_imp_included_asks in H2. eapply nodup_included_nodup in H2.
-all: exact. } Qed.
+Proof. { intros H. unfold matching in H. destruct H. destruct H0.
+         unfold matching. split. 
+         { eauto. }
+         split.
+         {  assert (H2: included (delete m M) (M)).
+            eapply included_elim4a. eapply included_M_imp_included_bids in H2.
+            eapply nodup_included_nodup in H2.
+            all: exact. }
+         { assert (H2: included (delete m M) (M)).
+           eapply included_elim4a. eapply included_M_imp_included_asks in H2.
+           eapply nodup_included_nodup in H2.
+           all: exact. } } Qed.
 
 Lemma matching_elim10 (m: fill_type) (M: list fill_type): matching M -> In m M ->
                                                           ~ In (bid_of m) (bids_of (delete m M)).
@@ -214,11 +234,13 @@ Proof. intros. eapply  matching_elim7. all: exact. Qed.
 
 Lemma matching_elim12 (m: fill_type) (M: list fill_type): matching (m::M) ->
                                                           ~ In (bid_of m) (bids_of M).
-Proof. intros. intro. destruct H. destruct H1.  simpl in H1. eapply nodup_elim2 in H1. contradiction. Qed.
+Proof. { intros. intro. destruct H. destruct H1.  simpl in H1.
+         eapply nodup_elim2 in H1. contradiction. } Qed.
 
 Lemma matching_elim13 (m: fill_type) (M: list fill_type): matching (m::M) ->
                                                           ~ In (ask_of m) (asks_of M).
-Proof. intros. intro. destruct H. destruct H1.  simpl in H2. eapply nodup_elim2 in H2. contradiction. Qed.
+Proof. { intros. intro. destruct H. destruct H1.  simpl in H2. eapply nodup_elim2 in H2.
+         contradiction. } Qed.
 
 
 
@@ -235,11 +257,13 @@ Lemma matching_in_intro (m: fill_type) (M: list fill_type)(B: list Bid)(A: list 
   (ask_of m) <= (bid_of m) -> matching_in B A M -> ~ In (bid_of m) (bids_of M) ->
   ~ In (ask_of m) (asks_of M) -> In (bid_of m) B -> In (ask_of m) A -> matching_in B A (m::M).
 
-Proof.  intros H1 H2 H3 H4 H5 H6. unfold matching_in. split. unfold matching in H2. destruct H2. destruct H. destruct H2. destruct H0. unfold matching.
-split. eauto. split. simpl. eapply nodup_intro in H3. exact. exact.
-eapply nodup_intro in H4. exact. exact. destruct H2. destruct H0. split.
-simpl. unfold "[<=]". intros. destruct H7. subst a. exact. eauto.
-simpl. unfold "[<=]". intros. destruct H7. subst a. exact. eauto. Qed.
+Proof.  { intros H1 H2 H3 H4 H5 H6. unfold matching_in. split.
+          unfold matching in H2. destruct H2. destruct H. destruct H2.
+          destruct H0. unfold matching.
+          split. eauto. split. simpl. eapply nodup_intro in H3. exact. exact.
+          eapply nodup_intro in H4. exact. exact. destruct H2. destruct H0. split.
+          simpl. unfold "[<=]". intros. destruct H7. subst a. exact. eauto.
+          simpl. unfold "[<=]". intros. destruct H7. subst a. exact. eauto. } Qed.
 
   Lemma matching_in_elim0 (M: list fill_type)(B: list Bid)(A: list Ask): matching_in B A M ->
                                                                          matching M.
@@ -248,12 +272,13 @@ simpl. unfold "[<=]". intros. destruct H7. subst a. exact. eauto. Qed.
   
 Lemma matching_in_elim (m: fill_type) (M: list fill_type)(B: list Bid)(A: list Ask):
   matching_in B A (m::M) -> matching_in B A M.
-  Proof. intros. unfold matching_in in H. destruct H. destruct H0. 
-  unfold matching_in. split. eauto. split. eauto. eauto. Qed.
+Proof. { intros. unfold matching_in in H. destruct H. destruct H0. 
+         unfold matching_in. split. eauto. split. eauto. eauto. } Qed.
 
 Lemma matching_in_elim1 (m: fill_type) (M: list fill_type) (B: list Bid)(A: list Ask):
   matching_in B A (m::M) ->  (ask_of m) <= (bid_of m).
-Proof. unfold matching_in. intros H. destruct H as [H1 H]. destruct H1 as [H1 H2]. eauto. Qed.
+Proof. { unfold matching_in. intros H. destruct H as [H1 H].
+         destruct H1 as [H1 H2]. eauto. } Qed.
  
 
 Lemma matching_in_elim2 (m: fill_type) (M: list fill_type) (B: list Bid)(A: list Ask):
@@ -295,21 +320,23 @@ Proof. intros. unfold matching_in in H. destruct H. destruct H1. eauto. Qed.
 
 Lemma matching_in_elim6 (a: Ask)(B: list Bid)(A: list Ask)(M: list fill_type):
   matching_in B A M -> matching_in B (a::A) M.
-Proof. unfold matching_in. intros. destruct H. destruct H0. split. exact.
- split. exact. eauto. Qed.
+Proof. { unfold matching_in. intros. destruct H. destruct H0. split. exact.
+         split. exact. eauto. } Qed.
 
 Lemma matching_in_elim7 (b: Bid)(B: list Bid)(A: list Ask)(M: list fill_type):
   matching_in B A M -> matching_in (b::B) A M.
-Proof. unfold matching_in. intros. destruct H. destruct H0. split. exact.
- split. eauto. exact. Qed.
+Proof. { unfold matching_in. intros. destruct H. destruct H0. split. exact.
+         split. eauto. exact. } Qed.
 
 
  Lemma matching_in_elim8 (B: list Bid)(A: list Ask)(b: Bid)(a: Ask)(M: list fill_type):
    matching_in (b::B) (a::A) M -> ~ In b (bids_of M) -> ~ In a (asks_of M) -> matching_in B A M.
- Proof. unfold matching_in. intros. destruct H. destruct H2. destruct H.
- destruct H4. unfold matching. split. { split. { exact. } { eauto. } }
-  split. { eapply subset_nodup_subset in H2. all: exact. }
-  { eapply subset_nodup_subset in H3. all: exact. } Qed.
+ Proof. { unfold matching_in. intros. destruct H. destruct H2. destruct H.
+          destruct H4. unfold matching. split.
+          { split. { exact. } { eauto. } }
+          split.
+          { eapply subset_nodup_subset in H2. all: exact. }
+          { eapply subset_nodup_subset in H3. all: exact. } } Qed.
 
 Hint Resolve matching_in_elim4a matching_in_elim5a: core. 
 Hint Immediate matching_in_intro: auction.
@@ -357,12 +384,18 @@ Definition Uniform (M : list fill_type) := uniform (trade_prices_of M).
 
 
 Lemma Uniform_intro (M:list fill_type) (m:fill_type) : Uniform M -> Uniform (delete m M).
-Proof. unfold Uniform. induction M. simpl. auto. intros H. simpl.  case (m_eqb m a) eqn: H1.  assert (H2:uniform (trade_prices_of M)). assert (H2: uniform (trade_prices_of (a :: M))). exact H. revert H2. eapply uniform_elim2. exact H2. simpl in H. eapply uniform_elim2 in H as H2.  eapply IHM in H2. simpl.  Admitted.
+Proof. { unfold Uniform. induction M. simpl. auto. intros H.
+         simpl.  case (m_eqb m a) eqn: H1.
+         assert (H2:uniform (trade_prices_of M)).
+         assert (H2: uniform (trade_prices_of (a :: M))).
+         exact H. revert H2. eapply uniform_elim2. exact H2.
+         simpl in H. eapply uniform_elim2 in H as H2.  eapply IHM in H2. simpl.  Admitted.
 
 Lemma Uniform_intro1 (M:list fill_type) (m:fill_type) : Uniform (m::M) -> Uniform M.
 Proof. unfold Uniform.  simpl.  eapply uniform_elim2. Qed.
 
-Lemma Uniform_elim (M:list fill_type) (m1 m2:fill_type) : Uniform M -> In m1 M -> In m2 M -> tp m1= tp m2.
+Lemma Uniform_elim (M:list fill_type) (m1 m2:fill_type) :
+  Uniform M -> In m1 M -> In m2 M -> tp m1= tp m2.
 Proof. Admitted.
 
 Lemma Uniform_intro2 (M:list fill_type) (m m':fill_type) : Uniform M -> 
